start updaing for Red

examples/pseudo_bool/array/pb_listScript.sml
@@ -5,28 +5,6 @@ open preamble basis pb_checkTheory;
 
 val _ = new_theory "pb_list"
 
-(* Make an array representation of a constraint *)
-Definition expand_constraint_aux_def:
-  (expand_constraint_aux [] (lit_arr:int list) = (lit_arr,[])) ∧
-  (expand_constraint_aux ((n,l)::xs) lit_arr =
-    let (lit_arr', vs') = expand_constraint_aux xs lit_arr in
-    case l of
-      Neg v =>
-      let la = update_resize lit_arr' 0 (-(&n)) v in (la,v::vs')
-    | Pos v =>
-      let la = update_resize lit_arr' 0 (&n) v in (la,v::vs'))
-End
-
-Definition contract_constraint_aux_def:
-  (contract_constraint_aux lit_arr [] = []) ∧
-  (contract_constraint_aux lit_arr (v::vs) =
-    let n = any_el v lit_arr 0 in
-    if n < 0 then
-      (Num (-n), Neg v) :: contract_constraint_aux lit_arr vs
-    else
-      (Num (n), Pos v) :: contract_constraint_aux lit_arr vs)
-End
-
 Theorem any_el_update_resize:
   any_el n (update_resize fml def v id) def =
   if n = id then v else any_el n fml def
@@ -36,84 +14,108 @@ Proof
   every_case_tac>>fs[]
 QED
 
-Theorem not_var_contract:
-  ∀vs la.
-  EVERY (\v.  v ≠ n) vs ⇒
-  contract_constraint_aux (update_resize la 0 q n) vs =
-  contract_constraint_aux la vs
-Proof
-  Induct>>
-  rw[]>>
-  simp[contract_constraint_aux_def]>>
-  simp[any_el_update_resize]
-QED
+(*
+  (* Make an array representation of a constraint *)
+  Definition expand_constraint_aux_def:
+    (expand_constraint_aux [] (lit_arr:int list) = (lit_arr,[])) ∧
+    (expand_constraint_aux ((n,l)::xs) lit_arr =
+      let (lit_arr', vs') = expand_constraint_aux xs lit_arr in
+      case l of
+        Neg v =>
+        let la = update_resize lit_arr' 0 (-(&n)) v in (la,v::vs')
+      | Pos v =>
+        let la = update_resize lit_arr' 0 (&n) v in (la,v::vs'))
+  End
 
-Theorem expand_constraint_get_var:
-  ∀xs lit_arr lit_arr' vs'.
-  expand_constraint_aux xs lit_arr = (lit_arr',vs') ⇒
-  vs' = MAP (get_var o SND) xs
-Proof
-  Induct>>fs[expand_constraint_aux_def]>>
-  Cases>>fs[expand_constraint_aux_def]>>rw[]>>
-  pairarg_tac>>fs[]>>
-  first_x_assum drule>>fs[]>>
-  every_case_tac>>fs[]>>rw[]
-QED
+  Definition contract_constraint_aux_def:
+    (contract_constraint_aux lit_arr [] = []) ∧
+    (contract_constraint_aux lit_arr (v::vs) =
+      let n = any_el v lit_arr 0 in
+      if n < 0 then
+        (Num (-n), Neg v) :: contract_constraint_aux lit_arr vs
+      else
+        (Num (n), Pos v) :: contract_constraint_aux lit_arr vs)
+  End
 
-Theorem contract_expand_constraint_aux:
-  ∀xs lit_arr lit_arr' vs'.
-  SORTED term_lt xs ∧
-  EVERY (λ(c,l). c ≠ 0) xs ∧
-  expand_constraint_aux xs lit_arr = (lit_arr',vs') ⇒
-  contract_constraint_aux lit_arr' vs' = xs
-Proof
-  Induct>>fs[expand_constraint_aux_def,contract_constraint_aux_def]>>
-  Cases>>rw[]>>
-  fs[expand_constraint_aux_def,contract_constraint_aux_def]>>
-  pairarg_tac>>fs[]>>
-  drule SORTED_TL>>
-  strip_tac>>
-  fs[]>>
-  first_x_assum drule>>
-  `EVERY (\v. get_var v ≠ get_var r) (MAP SND xs)` by
-    (simp[EVERY_MAP]>>
-    qpat_x_assum`SORTED _ (_::_)` mp_tac>>
-    DEP_ONCE_REWRITE_TAC[SORTED_EQ]>>
-    simp[pb_constraintTheory.transitive_term_lt]>>
-    simp[EVERY_MEM,FORALL_PROD]>>
+  Theorem not_var_contract:
+    ∀vs la.
+    EVERY (\v.  v ≠ n) vs ⇒
+    contract_constraint_aux (update_resize la 0 q n) vs =
+    contract_constraint_aux la vs
+  Proof
+    Induct>>
     rw[]>>
-    CCONTR_TAC>>fs[]>>
-    first_x_assum drule>>
-    simp[])>>
-  every_case_tac>>fs[]>>rw[]
-  >> ( (* two subgoals *)
     simp[contract_constraint_aux_def]>>
-    simp[any_el_update_resize]>>
-    match_mp_tac not_var_contract>>
-    drule expand_constraint_get_var>>
-    disch_then SUBST1_TAC>>
-    fs[EVERY_MAP])
-QED
+    simp[any_el_update_resize]
+  QED
 
-Definition expand_constraint_def:
-  (expand_constraint (PBC l n) lit_arr =
-    (n,expand_constraint_aux l lit_arr))
-End
+  Theorem expand_constraint_get_var:
+    ∀xs lit_arr lit_arr' vs'.
+    expand_constraint_aux xs lit_arr = (lit_arr',vs') ⇒
+    vs' = MAP (get_var o SND) xs
+  Proof
+    Induct>>fs[expand_constraint_aux_def]>>
+    Cases>>fs[expand_constraint_aux_def]>>rw[]>>
+    pairarg_tac>>fs[]>>
+    first_x_assum drule>>fs[]>>
+    every_case_tac>>fs[]>>rw[]
+  QED
 
-Definition contract_constraint_def:
-  (contract_constraint (n,lit_arr,vs) =
-    PBC (contract_constraint_aux lit_arr vs) n)
-End
+  Theorem contract_expand_constraint_aux:
+    ∀xs lit_arr lit_arr' vs'.
+    SORTED term_lt xs ∧
+    EVERY (λ(c,l). c ≠ 0) xs ∧
+    expand_constraint_aux xs lit_arr = (lit_arr',vs') ⇒
+    contract_constraint_aux lit_arr' vs' = xs
+  Proof
+    Induct>>fs[expand_constraint_aux_def,contract_constraint_aux_def]>>
+    Cases>>rw[]>>
+    fs[expand_constraint_aux_def,contract_constraint_aux_def]>>
+    pairarg_tac>>fs[]>>
+    drule SORTED_TL>>
+    strip_tac>>
+    fs[]>>
+    first_x_assum drule>>
+    `EVERY (\v. get_var v ≠ get_var r) (MAP SND xs)` by
+      (simp[EVERY_MAP]>>
+      qpat_x_assum`SORTED _ (_::_)` mp_tac>>
+      DEP_ONCE_REWRITE_TAC[SORTED_EQ]>>
+      simp[pb_constraintTheory.transitive_term_lt]>>
+      simp[EVERY_MEM,FORALL_PROD]>>
+      rw[]>>
+      CCONTR_TAC>>fs[]>>
+      first_x_assum drule>>
+      simp[])>>
+    every_case_tac>>fs[]>>rw[]
+    >> ( (* two subgoals *)
+      simp[contract_constraint_aux_def]>>
+      simp[any_el_update_resize]>>
+      match_mp_tac not_var_contract>>
+      drule expand_constraint_get_var>>
+      disch_then SUBST1_TAC>>
+      fs[EVERY_MAP])
+  QED
 
-Theorem contract_expand_constraint:
-  compact c ⇒
-  contract_constraint (expand_constraint c lit_arr) = c
-Proof
-  Cases_on`c`>>rw[expand_constraint_def]>>
-  Cases_on`expand_constraint_aux l lit_arr`>>rw[contract_constraint_def]>>
-  drule contract_expand_constraint_aux>>
-  metis_tac[]
-QED
+  Definition expand_constraint_def:
+    (expand_constraint (PBC l n) lit_arr =
+      (n,expand_constraint_aux l lit_arr))
+  End
+
+  Definition contract_constraint_def:
+    (contract_constraint (n,lit_arr,vs) =
+      PBC (contract_constraint_aux lit_arr vs) n)
+  End
+
+  Theorem contract_expand_constraint:
+    compact c ⇒
+    contract_constraint (expand_constraint c lit_arr) = c
+  Proof
+    Cases_on`c`>>rw[expand_constraint_def]>>
+    Cases_on`expand_constraint_aux l lit_arr`>>rw[contract_constraint_def]>>
+    drule contract_expand_constraint_aux>>
+    metis_tac[]
+  QED
+*)
 
 Definition check_cutting_list_def:
   (check_cutting_list (fml: npbc option list) (Id n) =
@@ -128,11 +130,15 @@ Definition check_cutting_list_def:
     else NONE) ∧
   (check_cutting_list fml (Sat c) =
     OPTION_MAP saturate (check_cutting_list fml c)) ∧
-  (check_cutting_list fml (Lit l) = SOME (PBC [(1,l)] 0)) ∧
+  (check_cutting_list fml (Lit l) =
+    case l of
+      Pos v => SOME (PBC [(1,v)] 0)
+    | Neg v => SOME (PBC [(-1,v)] 0)) ∧
   (check_cutting_list fml (Weak c var) =
     OPTION_MAP (λc. weaken c var) (check_cutting_list fml c))
 End
 
+(*
 (* Multiply an expanded constraint by k *)
 Definition left_multiply_aux_def:
   (left_multiply_aux (k:int) lit_arr [] = lit_arr) ∧
@@ -189,6 +195,7 @@ Proof
     cheat)>>
   cheat
 QED
+*)
 
 (* Copied from LPR *)
 val list_delete_list_def = Define`
@@ -212,6 +219,19 @@ Definition rollback_def:
     (MAP ($+id_start) (COUNT_LIST (id_end-id_start))) fml
 End
 
+Definition extract_clauses_list_def:
+  (extract_clauses_list f def fml [] acc = SOME (REVERSE acc)) ∧
+  (extract_clauses_list f def fml (cpf::pfs) acc =
+    case cpf of
+      (NONE,pf) => extract_clauses_list f def fml pfs ((NONE,pf)::acc)
+    | (SOME (INL n),pf) =>
+      (case any_el n fml NONE of
+        NONE => NONE
+      | SOME c => extract_clauses_list f def fml pfs ((SOME (subst f c),pf)::acc))
+    | (SOME (INR u),pf) =>
+      extract_clauses_list f def fml pfs ((SOME (subst f def),pf)::acc))
+End
+
 (*
   fml is represented by an array [...], where fml[i] is the i-th constraint
     when fml[i]=NONE (or i is out of range)
@@ -223,6 +243,27 @@ End
   T for Unsat
   F for Cont
 *)
+Theorem list_size_REVERSE:
+  list_size f (REVERSE ls) = list_size f ls
+Proof
+  Induct_on`ls`>>rw[]>>
+  simp[list_size_append,list_size_def]
+QED
+
+Theorem extract_clauses_list_list_size:
+  ∀pfs cpfs acc.
+  extract_clauses_list f c fml pfs acc = SOME cpfs ⇒
+  list_size (λx. list_size pbpstep_size (SND x)) cpfs <=
+  (list_size
+  (pair_size (option_size (full_sum_size (λx. x) one_size)) (list_size pbpstep_size)) pfs) +
+  list_size (λx. list_size pbpstep_size (SND x)) (REVERSE acc)
+Proof
+  Induct>>rw[extract_clauses_list_def] >>simp[]>>
+  every_case_tac>>fs[]>>first_x_assum drule>>
+  simp[list_size_REVERSE]>>
+  EVAL_TAC>>simp[]
+QED
+
 Definition check_pbpstep_list_def:
   (check_pbpstep_list (step:pbpstep) (fml: npbc option list) (inds:num list) (mindel:num) (id:num) =
   case step of
@@ -250,23 +291,52 @@ Definition check_pbpstep_list_def:
       SOME (update_resize fml NONE (SOME c) id, F, (id+1), sorted_insert id inds))
   | Con c pf =>
     let fml_not_c = update_resize fml NONE (SOME (not c)) id in
-    (case check_pbpsteps_list pf fml_not_c inds id (id+1) of
+    (case check_pbpsteps_list pf fml_not_c (sorted_insert id inds) id (id+1) of
       SOME (fml', T, id' ,inds') =>
         let rfml = rollback fml' id id' in
         SOME(update_resize rfml NONE (SOME c) id', F, (id'+1), sorted_insert id' inds')
     | _ => NONE)
-  | _ => NONE) ∧
+  | Red c s pfs =>
+    (let fml_not_c = update_resize fml NONE (SOME (not c)) id in
+     let w = subst_fun s in
+      case extract_clauses_list w c fml pfs [] of
+        NONE => NONE
+      | SOME cpfs =>
+        case check_redundancy_list cpfs fml_not_c (sorted_insert id inds) id (id+1) of
+          SOME(fml', id', inds') =>
+          let rfml = rollback fml' id id' in
+          (* TODO: check that all goals are covered *)
+          SOME(update_resize rfml NONE (SOME c) id', F, (id'+1), sorted_insert id' inds')
+        | NONE => NONE
+       )) ∧
   (check_pbpsteps_list [] fml inds mindel id = SOME (fml, F, id, inds)) ∧
   (check_pbpsteps_list (step::steps) fml inds mindel id =
     case check_pbpstep_list step fml inds mindel id of
       SOME (fml', F, id', inds') =>
         check_pbpsteps_list steps fml' inds' mindel id'
-    | res => res)
+    | res => res) ∧
+  (check_redundancy_list [] fml inds mindel id = SOME(fml,id,inds)) ∧
+  (check_redundancy_list ((copt,pf)::pfs) fml inds mindel id =
+    case copt of
+      NONE => (* no clause given *)
+      (if ~EVERY is_pol_con pf then NONE else
+      case check_pbpsteps_list pf fml inds mindel id of
+        SOME (fml', F, id', inds') => check_redundancy_list pfs fml' inds' mindel id'
+      | res => NONE)
+    | SOME c =>
+      let cfml = update_resize fml NONE (SOME (not c)) id in
+      case check_pbpsteps_list pf cfml (sorted_insert id inds) mindel (id+1) of
+        SOME (fml', T, id', inds') =>
+        let rfml = rollback fml' id id' in
+          check_redundancy_list pfs rfml inds' mindel id'
+      | _ => NONE)
 Termination
   WF_REL_TAC ‘measure (
     sum_size (pbpstep_size o FST)
-    (list_size pbpstep_size o FST))’
+    (sum_size (list_size pbpstep_size o FST) (list_size (list_size pbpstep_size o SND) o FST)))’
   \\ fs [pbpstep_size_eq] \\ rw []
+  \\ drule extract_clauses_list_list_size
+  \\ simp[list_size_def]
 End
 
 (* TODO:
@@ -322,9 +392,18 @@ End
  *)
 
 (* prove that check_pbpstep_list implements check_pbpstep *)
+
+(* Relate sptree representation fml with list representation fmlls *)
 Definition fml_rel_def:
   fml_rel fml fmlls ⇔
   ∀x. any_el x fmlls NONE = lookup x fml
+End
+
+(* Index list must overapproximate active indices in fmlls *)
+Definition ind_rel_def:
+  ind_rel fmlls inds ⇔
+  ∀x. x < LENGTH fmlls ∧ IS_SOME (EL x fmlls) ⇒
+  MEM x inds
 End
 
 Theorem fml_rel_check_cutting:
@@ -333,7 +412,8 @@ Theorem fml_rel_check_cutting:
   check_cutting_list fmlls p = check_cutting fml p
 Proof
   Induct>>rw[check_cutting_list_def,check_cutting_def]>>
-  fs[fml_rel_def]
+  fs[fml_rel_def]>>
+  every_case_tac>>simp[check_cutting_def]
 QED
 
 Theorem any_el_list_delete_list:
@@ -369,22 +449,27 @@ Proof
   rw[fml_rel_def,lookup_insert,any_el_update_resize]
 QED
 
+(* id numbers are monotone increasing *)
 Theorem check_pbpstep_list_id:
   (∀step fmlls inds mindel id fmlls' b id' inds'.
   check_pbpstep_list step fmlls inds mindel id = SOME (fmlls', b,id',inds') ⇒ id ≤ id') ∧
   (∀steps fmlls inds mindel id fmlls' b id' inds'.
-  check_pbpsteps_list steps fmlls inds mindel id = SOME (fmlls', b,id',inds') ⇒ id ≤ id')
+  check_pbpsteps_list steps fmlls inds mindel id = SOME (fmlls', b,id',inds') ⇒ id ≤ id') ∧
+  (∀pfs fmlls inds mindel id fmlls' id' inds'.
+  check_redundancy_list pfs fmlls inds mindel id = SOME (fmlls',id',inds') ⇒ id ≤ id')
 Proof
   ho_match_mp_tac check_pbpstep_list_ind>>
   rw[]
-  >-
-    gvs [AllCaseEqs(),check_pbpstep_def,check_pbpstep_list_def]
-  >-
-    gvs [AllCaseEqs(),check_pbpstep_def,check_pbpstep_list_def]
+  >- gvs [AllCaseEqs(),check_pbpstep_def,check_pbpstep_list_def]
+  >- gvs [AllCaseEqs(),check_pbpstep_def,check_pbpstep_list_def]
+  >- gvs [AllCaseEqs(),check_pbpstep_def,check_pbpstep_list_def]
+  >- gvs [AllCaseEqs(),check_pbpstep_def,check_pbpstep_list_def]
   >- (
     pop_assum mp_tac>>
     simp[Once check_pbpstep_list_def,AllCaseEqs()] >>
-    rw[]>>first_x_assum drule>>
+    rw[]>>
+    fs[o_DEF,ETA_AX]>>
+    first_x_assum drule>>
     simp[]>>
     rw[]>>
     first_x_assum drule>>
@@ -392,6 +477,7 @@ Proof
     fs[])
 QED
 
+(* id numbers bound those in the formula *)
 Theorem check_pbpstep_list_id_upper:
   (∀step fmlls inds mindel id fmlls' b id' inds'.
   check_pbpstep_list step fmlls inds mindel id = SOME (fmlls', b,id',inds') ∧
@@ -400,20 +486,25 @@ Theorem check_pbpstep_list_id_upper:
   (∀steps fmlls inds mindel id fmlls' b id' inds'.
   check_pbpsteps_list steps fmlls inds mindel id = SOME (fmlls', b,id',inds') ∧
   (∀n. n ≥ id ⇒ any_el n fmlls NONE = NONE) ⇒
+  (∀n. n ≥ id' ⇒ any_el n fmlls' NONE = NONE)) ∧
+  (∀pfs fmlls inds mindel id fmlls' id' inds'.
+  check_redundancy_list pfs fmlls inds mindel id = SOME (fmlls',id',inds') ∧
+  (∀n. n ≥ id ⇒ any_el n fmlls NONE = NONE) ⇒
   (∀n. n ≥ id' ⇒ any_el n fmlls' NONE = NONE))
 Proof
   ho_match_mp_tac check_pbpstep_list_ind>>
   rw[]
-  >- (
+  >- ( (* slow *)
     gvs [AllCaseEqs(),check_pbpstep_def,check_pbpstep_list_def]
     >-
       simp[any_el_list_delete_list]
     >-
       simp[any_el_update_resize]
     >-
+      simp[any_el_update_resize,rollback_def,any_el_list_delete_list]
+    >-
       simp[any_el_update_resize,rollback_def,any_el_list_delete_list])
-  >-
-    gvs [AllCaseEqs(),check_pbpstep_def,check_pbpstep_list_def]
+  >- gvs [AllCaseEqs(),check_pbpstep_def,check_pbpstep_list_def]
   >- (
     qpat_x_assum`_= SOME _ `mp_tac>>
     simp[Once check_pbpstep_list_def,AllCaseEqs()] >>
@@ -424,17 +515,32 @@ Proof
     first_x_assum drule>>
     disch_then drule>>
     rw[])
+  >- gs[check_pbpstep_list_def]
+  >- (
+    qpat_x_assum`_= SOME _ `mp_tac>>
+    simp[Once check_pbpstep_list_def,AllCaseEqs()] >>
+    simp[o_DEF,ETA_AX]>>
+    rw[]>>first_x_assum drule
+    >- (
+      disch_then drule>> disch_then drule>>
+      rfs[])>>
+    rfs[]>>
+    fs[any_el_update_resize,rollback_def,any_el_list_delete_list])
 QED
 
 Theorem check_pbpstep_list_mindel:
   (∀step fmlls inds mindel id fmlls' res n.
-  check_pbpstep_list step fmlls inds mindel id = SOME (fmlls', res) ∧
-  mindel ≤ id ∧
-  n < mindel ⇒ any_el n fmlls NONE = any_el n fmlls' NONE) ∧
+    check_pbpstep_list step fmlls inds mindel id = SOME (fmlls', res) ∧
+    mindel ≤ id ∧
+    n < mindel ⇒ any_el n fmlls NONE = any_el n fmlls' NONE) ∧
   (∀steps fmlls inds mindel id fmlls' res n.
-  check_pbpsteps_list steps fmlls inds mindel id = SOME (fmlls', res) ∧
-  mindel ≤ id ∧
-  n < mindel ⇒ any_el n fmlls NONE = any_el n fmlls' NONE)
+    check_pbpsteps_list steps fmlls inds mindel id = SOME (fmlls', res) ∧
+    mindel ≤ id ∧
+    n < mindel ⇒ any_el n fmlls NONE = any_el n fmlls' NONE) ∧
+  (∀pfs fmlls inds mindel id fmlls' res n.
+    check_redundancy_list pfs fmlls inds mindel id = SOME (fmlls', res) ∧
+    mindel ≤ id ∧
+    n < mindel ⇒ any_el n fmlls NONE = any_el n fmlls' NONE)
 Proof
   ho_match_mp_tac check_pbpstep_list_ind>>
   rw[]
@@ -449,6 +555,11 @@ Proof
       first_x_assum(qspec_then`n`mp_tac)>>
       simp[any_el_update_resize]>>
       drule (el 2 (CONJUNCTS check_pbpstep_list_id))>>
+      simp[rollback_def,any_el_list_delete_list,MEM_MAP])
+    >- (
+      first_x_assum(qspec_then`n`mp_tac)>>
+      simp[any_el_update_resize]>>
+      drule (el 3 (CONJUNCTS check_pbpstep_list_id))>>
       simp[rollback_def,any_el_list_delete_list,MEM_MAP]))
   >-
     fs[check_pbpstep_list_def]
@@ -464,6 +575,21 @@ Proof
     disch_then (qspec_then`n`mp_tac)>>
     drule (el 1 (CONJUNCTS check_pbpstep_list_id))>>
     simp[])
+  >- fs[check_pbpstep_list_def]
+  >- (
+    qpat_x_assum`_=SOME _` mp_tac>>
+    simp[Once check_pbpstep_list_def,AllCaseEqs()] >>
+    simp[o_DEF,ETA_AX]>>
+    rw[]>>first_x_assum drule>>
+    rfs[]
+    >- (
+      rw[]>>
+      drule (el 2 (CONJUNCTS check_pbpstep_list_id))>>
+      fs[])>>
+    disch_then drule >>
+    rfs[any_el_update_resize,rollback_def,any_el_list_delete_list,MEM_MAP]>>
+    drule (el 2 (CONJUNCTS check_pbpstep_list_id))>>
+    fs[])
 QED
 
 Theorem fml_rel_rollback:
@@ -485,9 +611,155 @@ Proof
     metis_tac[])
 QED
 
+Theorem list_delete_list_FOLDL:
+  ∀l fmlls.
+  list_delete_list l fmlls =
+  FOLDL (\fml i.
+    if LENGTH fml ≤ i then fml else LUPDATE NONE i fml) fmlls l
+Proof
+  Induct>>rw[list_delete_list_def]
+QED
+
+Theorem ind_rel_list_delete_list:
+  ∀l fmlls.
+  ind_rel fmlls inds ==>
+  ind_rel (list_delete_list l fmlls) inds
+Proof
+  simp[list_delete_list_FOLDL,FOLDL_FOLDR_REVERSE]>>
+  strip_tac>>
+  qabbrev_tac`ll= REVERSE l`>>
+  pop_assum kall_tac>>
+  Induct_on`ll`>>
+  rw[]>>fs[]>>
+  first_x_assum drule>>
+  rw[ind_rel_def,EL_LUPDATE]>>
+  pop_assum mp_tac>> IF_CASES_TAC>>fs[]
+QED
+
+
+Theorem ind_rel_update_resize:
+  ind_rel fmlls inds ⇒
+  ind_rel (update_resize fmlls NONE v n) (n::inds)
+Proof
+  rw[update_resize_def,ind_rel_def,EL_LUPDATE]>>every_case_tac>>fs[]>>
+  fs[ind_rel_def]>>rw[]>>
+  fs[IS_SOME_EXISTS,EL_APPEND_EQN]>>
+  every_case_tac>>fs[]>>
+  rfs[EL_REPLICATE,LENGTH_REPLICATE]
+QED
+
+Theorem MEM_sorted_insert:
+  ∀ls.
+  MEM y (sorted_insert n ls) <=> MEM y (n::ls)
+Proof
+  Induct>>rw[sorted_insert_def]>>fs[]>>
+  metis_tac[]
+QED
+
+Theorem SORTED_sorted_insert:
+  ∀ls.
+  SORTED $>= ls ⇒
+  SORTED $>= (sorted_insert n ls)
+Proof
+  Induct>>rw[sorted_insert_def]>>
+  pop_assum mp_tac>>
+  DEP_REWRITE_TAC [SORTED_EQ]>>
+  simp[transitive_def]>>
+  rw[]>>
+  fs[MEM_sorted_insert]>>rw[]
+QED
+
+Theorem ind_rel_update_resize_sorted_insert:
+  ind_rel fmlls inds ⇒
+  ind_rel (update_resize fmlls NONE v n) (sorted_insert n inds)
+Proof
+  strip_tac>> drule ind_rel_update_resize>>
+  metis_tac[ind_rel_def,MEM_sorted_insert]
+QED
+
+Theorem ind_rel_update_resize:
+  ind_rel fmlls inds ⇒
+  ind_rel (update_resize fmlls NONE v n) (n::inds)
+Proof
+  rw[update_resize_def,ind_rel_def,EL_LUPDATE]>>every_case_tac>>fs[]>>
+  fs[ind_rel_def]>>rw[]>>
+  fs[IS_SOME_EXISTS,EL_APPEND_EQN]>>
+  every_case_tac>>fs[]>>
+  rfs[EL_REPLICATE,LENGTH_REPLICATE]
+QED
+
+Theorem MEM_sorted_insert:
+  ∀ls.
+  MEM y (sorted_insert n ls) <=> MEM y (n::ls)
+Proof
+  Induct>>rw[sorted_insert_def]>>fs[]>>
+  metis_tac[]
+QED
+
+Theorem SORTED_sorted_insert:
+  ∀ls.
+  SORTED $>= ls ⇒
+  SORTED $>= (sorted_insert n ls)
+Proof
+  Induct>>rw[sorted_insert_def]>>
+  pop_assum mp_tac>>
+  DEP_REWRITE_TAC [SORTED_EQ]>>
+  simp[transitive_def]>>
+  rw[]>>
+  fs[MEM_sorted_insert]>>rw[]
+QED
+
+Theorem ind_rel_update_resize_sorted_insert:
+  ind_rel fmlls inds ⇒
+  ind_rel (update_resize fmlls NONE v n) (sorted_insert n inds)
+Proof
+  strip_tac>> drule ind_rel_update_resize>>
+  metis_tac[ind_rel_def,MEM_sorted_insert]
+QED
+
+Theorem ind_rel_rollback:
+  ind_rel fmlls inds ⇒
+  ind_rel (rollback fmlls id id') inds
+Proof
+  rw[rollback_def]>>
+  metis_tac[ind_rel_list_delete_list]
+QED
+
+Theorem ind_rel_check_pbpstep_list:
+  (∀step fmlls inds mindel id fmlls' b id' inds' fml.
+  ind_rel fmlls inds ∧
+  check_pbpstep_list step fmlls inds mindel id = SOME (fmlls', b,id',inds') ⇒
+  ind_rel fmlls' inds') ∧
+  (∀steps fmlls inds mindel id fmlls' b id' inds' fml.
+  ind_rel fmlls inds ∧
+  check_pbpsteps_list steps fmlls inds mindel id = SOME (fmlls', b,id',inds') ⇒
+  ind_rel fmlls' inds') ∧
+  (∀pfs fmlls inds mindel id fmlls' id' inds' fml.
+  ind_rel fmlls inds ∧
+  check_redundancy_list pfs fmlls inds mindel id = SOME (fmlls', id',inds') ⇒
+  ind_rel fmlls' inds')
+Proof
+  ho_match_mp_tac check_pbpstep_list_ind>>
+  rw[]
+  >- (
+    gvs [AllCaseEqs(),check_pbpstep_def,check_pbpstep_list_def]
+    >- metis_tac[ind_rel_list_delete_list]
+    >- metis_tac[ind_rel_update_resize_sorted_insert]
+    >- metis_tac[ind_rel_update_resize_sorted_insert,ind_rel_rollback]
+    >- metis_tac[ind_rel_update_resize_sorted_insert,ind_rel_rollback])
+  >- fs[check_pbpstep_list_def]
+  >- gvs [AllCaseEqs(),check_pbpstep_list_def]
+  >- gvs [AllCaseEqs(),check_pbpstep_list_def]
+  >- (
+    gvs [AllCaseEqs(),check_pbpstep_list_def]>>
+    fs[o_DEF,ETA_AX]>>
+    metis_tac[ind_rel_update_resize_sorted_insert,ind_rel_rollback])
+QED
+
 Theorem fml_rel_check_pbpstep_list:
   (∀step fmlls inds mindel id fmlls' b id' inds' fml.
   fml_rel fml fmlls ∧
+  ind_rel fmlls inds ∧
   (∀n. n ≥ id ⇒ any_el n fmlls NONE = NONE) ∧
   mindel ≤ id ∧
   check_pbpstep_list step fmlls inds mindel id = SOME (fmlls', b,id',inds') ⇒
@@ -495,12 +767,23 @@ Theorem fml_rel_check_pbpstep_list:
   else ∃fml'. check_pbpstep step fml id = Cont fml' id' ∧ fml_rel fml' fmlls') ∧
   (∀steps fmlls inds mindel id fmlls' b id' inds' fml.
   fml_rel fml fmlls ∧
+  ind_rel fmlls inds ∧
+  (∀n. n ≥ id ⇒ any_el n fmlls NONE = NONE) ∧
   (∀n. n ≥ id ⇒ any_el n fmlls NONE = NONE) ∧
   mindel ≤ id ∧
   check_pbpsteps_list steps fmlls inds mindel id = SOME (fmlls', b,id',inds') ⇒
   if b then check_pbpsteps steps fml id = Unsat id'
-  else ∃fml'. check_pbpsteps steps fml id = Cont fml' id' ∧ fml_rel fml' fmlls')
+  else ∃fml'. check_pbpsteps steps fml id = Cont fml' id' ∧ fml_rel fml' fmlls') ∧
+  (∀pfs fmlls inds mindel id fmlls' id' inds' fml.
+  fml_rel fml fmlls ∧
+  ind_rel fmlls inds ∧
+  (∀n. n ≥ id ⇒ any_el n fmlls NONE = NONE) ∧
+  mindel ≤ id ∧
+  check_redundancy_list pfs fmlls inds mindel id = SOME (fmlls', id',inds') ⇒
+  ∃fml'. check_redundancy pfs fml id = Cont fml' id' ∧ fml_rel fml' fmlls')
 Proof
+  cheat
+  (*
   ho_match_mp_tac check_pbpstep_list_ind>>
   rw[]
   >- (
@@ -555,7 +838,7 @@ Proof
         disch_then match_mp_tac>>fs[])
       >- (strip_tac>>simp[Once check_pbpstep_def])>>
       strip_tac>>simp[Once check_pbpstep_def])
-    )
+    ) *)
 QED
 
 val _ = export_theory();
